WIP

src/tlogic/LiveObligations.v
@@ -10,7 +10,6 @@ From Fairness Require Export ObligationRA SimDefaultRA.
 Require Export Nat.
 
 Notation "'ω'" := Ord.omega.
-(* Notation "'ω'" := Ord.omega : ord_scope. *)
 
 Section LAYER.
 
@@ -210,8 +209,17 @@ Section RULES.
   Definition progress_credit (k : nat) (l a : nat) :=
     white k (layer l a).
 
+  Definition pending_obligation (k : nat) (q : Qp) :=
+    (pending k q)%I.
+
+  Definition active_obligation (k : nat) :=
+    (shot k)%I.
+
   Global Program Instance Persistent_liveness_obligation k l :
     Persistent (liveness_obligation k l).
+
+  Global Program Instance Persistent_active_obligation k :
+    Persistent (active_obligation k).
 
   Lemma lo_mon k l1 l2 :
     (l1 <= l2) ->
@@ -284,9 +292,9 @@ Section RULES.
   Qed.
 
   Lemma alloc_obligation l a :
-    ⊢ |==> (∃ k, liveness_obligation k l ∗ progress_credit k l a).
+    ⊢ |==> (∃ k, liveness_obligation k l ∗ progress_credit k l a ∗ pending_obligation k 1).
   Proof.
-    iMod (alloc (layer l a)) as "[% [B W]]".
+    iMod (alloc (layer l a)) as "[% (B & W & P)]".
     iExists k. iFrame. iModIntro. iExists a, (layer l a). iFrame.
     auto.
   Qed.
@@ -351,11 +359,38 @@ Section RULES.
 
   Definition fairness_credit {Id} (p : Prism.t _ Id) (i : Id) : iProp := FairRA.white p i 1.
 
+  Definition delayed_promise {Id} {v} (p : Prism.t _ Id) (i : Id) k l f : iProp :=
+    delay v p i k (layer l 1) f.
+
   Definition promise {Id} {v} (p : Prism.t _ Id) (i : Id) k l f : iProp :=
     correl v p i k (layer l 1) f.
 
+  Global Program Instance Persistent_delayed_promise {Id} {v} p (i : Id) k l f :
+    Persistent (delayed_promise (v:=v) p i k l f).
+
   Global Program Instance Persistent_promise {Id} {v} p (i : Id) k l f :
     Persistent (promise (v:=v) p i k l f).
+
+  Lemma activate_promise {Id} {v} (p : Prism.t _ Id) (i : Id) k c (F : Vars v)
+    :
+    (delayed_promise p i k c F)
+      -∗
+      (pending_obligation k (1/2))
+      -∗
+      (#=(arrows_sat v)=> (promise p i k c F) ∗ (active_obligation k)).
+  Proof.
+    iIntros "#DP PO". iMod (delay_shot with "DP PO") as "[_ #S]".
+    iPoseProof (delay_to_correl with "DP S") as "P". iModIntro. auto.
+  Qed.
+
+  Lemma unfold_promise {Id} {v} (p : Prism.t _ Id) (i : Id) k c (F : Vars v)
+    :
+    (promise p i k c F)
+      -∗
+      (delayed_promise p i k c F ∗ active_obligation k).
+  Proof.
+    iIntros "P". iPoseProof (unfold_correl with "P") as "A". iFrame.
+  Qed.
 
   Lemma promise_progress {Id} {v} (p : Prism.t _ Id) (i : Id) k l f :
     (promise p i k l f ∗ fairness_credit p i)
@@ -365,16 +400,24 @@ Section RULES.
   Qed.
 
   Lemma duty_add {Id} {v} (p : Prism.t _ Id) (i : Id) ds k l f :
-    (duty p i ds ∗ progress_credit k (1 + l) 1)
+    (duty p i ds ∗ progress_credit k (1 + l) 1 ∗ pending_obligation k (1/2))
       ⊢ (□ (prop v f -∗ □ prop v f)) =(arrows_sat v)=∗ duty p i ((k, l, f) :: ds).
   Proof.
-    iIntros "[D PC] #F". iMod (duty_alloc with "D [PC] [F]") as "D".
+    iIntros "[D [PC PO]] #F". iMod (duty_alloc with "D [PC] PO [F]") as "D".
     { unfold progress_credit. iPoseProof (white_eq with "PC") as "PC".
       { replace (1+l) with (l+1) by lia. rewrite layer_sep. rewrite layer_one_one. reflexivity. }
       iFrame.
     }
     { eauto. }
     iModIntro. iFrame.
+  Qed.
+
+  Lemma duty_delayed_promise {Id} {v} (p : Prism.t _ Id) (i : Id) ds k l (f : Vars v) :
+    In (k, l, f) ds ->
+    duty p i ds ⊢ promise p i k l f.
+  Proof.
+    iIntros (IN) "D". iApply duty_correl. 2: iFrame.
+    apply (in_map (fun '(k0, l0, f0) => (k0, layer l0 1, f0))) in IN. auto.
   Qed.
 
   Lemma duty_promise {Id} {v} (p : Prism.t _ Id) (i : Id) ds k l (f : Vars v) :
